Make Dafny AWS KMS client suppliers natively return AWS KMS clients

src/api/dotnet/AWSKMSClientSuppliers.cs
@@ -1,3 +1,4 @@
+using System;
 using System.Collections.Generic;
 using System.Linq;
 using icharseq = Dafny.ISequence<char>;
@@ -8,6 +9,14 @@ namespace AWSEncryptionSDK
 {
     public interface AWSKMSClientSupplier {
         AmazonKeyManagementServiceClient GetClient(string region);
+    }
+
+    public class AWSKMSClientSupplierException : Exception
+    {
+        public AWSKMSClientSupplierException(string msg)
+            : base(msg)
+        {
+        }
     }
 
     public class AWSKMSClientSuppliers {
@@ -23,35 +32,39 @@ namespace AWSEncryptionSDK
             // instantiate the class and then manually call __ctor() to call the required constructor
             KMSUtils.BaseClientSupplier clientSupplier = new KMSUtils.BaseClientSupplier();
             clientSupplier.__ctor();
-            return clientSupplier;
+            return new KMSUtils.DafnyAWSKMSClientSupplierWrapper(clientSupplier);
         }
 
         // An implementation of an AWSKMSClientSupplier that takes in an existing AWSKMSClientSupplier as well as an
-        // enumerable of region strings. The LimitRegionsClientSupplier will only return an AWSKMSClient from the given
-        // AWSKMSClientSupplier if the region provided to GetClient(region) is in the list of regions associated with
-        // the LimitRegionsClientSupplier.
+        // enumerable of region strings. The LimitRegionsClientSupplier will only return an AWS KMS service client from
+        // the given AWSKMSClientSupplier if the region provided to GetClient(region) is in the list of regions
+        // associated with the LimitRegionsClientSupplier.
         public static AWSKMSClientSupplier NewKMSLimitRegionsClientSupplier(AWSKMSClientSupplier clientSupplier, IEnumerable<string> regions)
         {
             // When transpiling Dafny code, new MyClass() does not actually call the constructor, so we need to
             // instantiate the class and then manually call __ctor() to call the required constructor
             KMSUtils.LimitRegionsClientSupplier limitRegionsclientSupplier = new KMSUtils.LimitRegionsClientSupplier();
             var convertedRegions = regions.Select(DafnyFFI.DafnyStringFromString).ToArray();
-            limitRegionsclientSupplier.__ctor(clientSupplier, Dafny.Sequence<icharseq>.FromElements(convertedRegions));
-            return limitRegionsclientSupplier;
+            limitRegionsclientSupplier.__ctor(
+                new KMSUtils.AWSKMSClientSupplierWrapper(clientSupplier),
+                Dafny.Sequence<icharseq>.FromElements(convertedRegions));
+            return new KMSUtils.DafnyAWSKMSClientSupplierWrapper(limitRegionsclientSupplier);
         }
 
         // An implementation of an AWSKMSClientSupplier that takes in an existing AWSKMSClientSupplier as well as an
-        // enumerable of region strings. The ExcludeRegionsClientSupplier will only return an AWSKMSClient from the given
-        // AWSKMSClientSupplier if the region provided to GetClient(region) is not in the list of regions associated with
-        // the ExcludeRegionsClientSupplier.
+        // enumerable of region strings. The ExcludeRegionsClientSupplier will only return an AWS KMS service client from
+        // the given AWSKMSClientSupplier if the region provided to GetClient(region) is not in the list of regions
+        // associated with the ExcludeRegionsClientSupplier.
         public static AWSKMSClientSupplier NewKMSExcludeRegionsClientSupplier(AWSKMSClientSupplier clientSupplier, IEnumerable<string> regions)
         {
             // When transpiling Dafny code, new MyClass() does not actually call the constructor, so we need to
             // instantiate the class and then manually call __ctor() to call the required constructor
             KMSUtils.ExcludeRegionsClientSupplier excludeRegionsclientSupplier = new KMSUtils.ExcludeRegionsClientSupplier();
             var convertedRegions = regions.Select(DafnyFFI.DafnyStringFromString).ToArray();
-            excludeRegionsclientSupplier.__ctor(clientSupplier, Dafny.Sequence<icharseq>.FromElements(convertedRegions));
-            return excludeRegionsclientSupplier;
+            excludeRegionsclientSupplier.__ctor(
+                new KMSUtils.AWSKMSClientSupplierWrapper(clientSupplier),
+                Dafny.Sequence<icharseq>.FromElements(convertedRegions));
+            return new KMSUtils.DafnyAWSKMSClientSupplierWrapper(excludeRegionsclientSupplier);
         }
     }
 }
